Main.lean
@@ -3,8 +3,10 @@ import «EventSystems».Convergent
 import «EventSystems».NonDet.Basic
 import «EventSystems».NonDet.Convergent
 import «EventSystems».Refinement.Basic
+import «EventSystems».Refinement.Convergent
 
 import «Examples».EventB.Bridge.Bridge0
+import «Examples».EventB.Bridge.Bridge1
 
 
 
